

Q 5 ...

$$p(x) y'' + q(x) y' + r(x) y = 0$$

$$\lim_{x \rightarrow 0} x \frac{q(x)}{p(x)}$$

(2)

$$\lim_{x \rightarrow 0} x^2 \frac{2 dx}{p(x)}$$

-2

$$p(x) = x^2$$

$$p(0) = 0$$

$$y = \sum_{n=0}^{\infty} a_n x^{n+r}$$

$$y' = \left( \sum_{n=0}^{\infty} a_n x^{n+r} \right)' = \left( \sum_{n=0}^{\infty} a_n (n+r) x^{n+r-1} \right)'$$

$$a_n (n+r) x^{n+r-1}$$

$$y' = \sum_{n=0}^{\infty} a_n (n+r) x^{n+r-1}$$

$$y'' = \sum_{n=0}^{\infty} a_n (n+r) (n+r-1) x^{n+r-2}$$

Sena ERSOY  
06.02.2004 34

$$x^2 \sum_0^{\infty} a_n(n+r)(n+r-1)x^{n+r-2} + (2x + 3x^2).$$

$$\sum_0^{\infty} a_n(n+r)x^{n+r-1} - 2 \sum_0^{\infty} a_n x^{n+r} = 0$$

$$= \sum_0^{\infty} a_n(2nr + r^2 - r + n^2 - n)x^{n+r} + \sum_0^{\infty} 3a_n(n+r)x^{n+r+1} + \sum_0^{\infty} 2a_n(n+r)x^{n+r} - \sum_0^{\infty} 2a_n x^{n+r}$$

$$= (2a_0r^2 + 2a_0r - 2a_0)x^r + \sum_{n=1}^{\infty} (a_n r^2 + 2a_n r + 3a_{n-1}r + 2a_n n r - 2a_n - 3a_{n-1} + a_n n^2 + a_n n + 3a_{n-1}n)x^{n+r}$$

$$+ 2a_n n r - 2a_n - 3a_{n-1} + a_n n^2 + a_n n + 3a_{n-1}n)x^{n+r}$$

$$\rightarrow = 0 \rightarrow r_1 = -1 \quad r_2 = 1$$

$$(a_0 + a_0 - 2a_0)x + \sum_1^{\infty} (a_n + a_n + 3a_{n-1} + 2a_n n - 2a_n - 3a_{n-1} + a_n n^2 + a_n n + 3a_{n-1}n)x^{n+1} = 0$$

$$\sum_1^{\infty} (n^2 a_n + 3n a_n + 3n a_{n-1})x^{n+1}$$

$$(n^2 a_n + 3n a_n + 3n a_{n-1}) = 0 \quad a_n = -\frac{3a_{n-1}}{n+3}$$

$$a_1 = -\frac{3a_0}{4}$$

$$a_2 = -\frac{3a_1}{5} = \frac{9a_0}{20}$$

$$a_3 = \frac{3a_2}{6} = \frac{3 \cdot 9}{6 \cdot 20} a_0 \dots$$

$$y_1 = a_0 x \left( 1 - \frac{3x}{4} + \frac{9x^2}{20} + \dots \right)$$

$$y_1 = c_1 x \left( 1 - \frac{3x}{4} + \frac{9x^2}{20} \dots \right)$$

Sena ERS04

040200434

Handwritten signature